modified encoding of choice operator and updated proofs

FiatFormal/Language/Step.v
@@ -2,6 +2,7 @@
 Require Import FiatFormal.Language.SubstTypeExp.
 Require Import FiatFormal.Language.SubstExpExp.
 Require Export FiatFormal.Language.Exp.
+Require Import FiatFormal.Language.TyJudge.
 
 Require Export FiatFormal.Language.Context.
 
@@ -59,33 +60,44 @@ Inductive exp_ctx : (exp -> exp) -> Prop :=
      value v1
      -> exps_ctx wnfX C
      -> exp_ctx (fun xx => XNApp v1 (C xx)).
-
 Hint Constructors exp_ctx.
 
-Inductive STEP : exp -> exp -> Prop :=
+
+Inductive STEP
+          (ProofBuilder : propcon -> list exp -> Prop)
+          (ds : defs)
+          (ProofBuilderOK : forall ke te pc xs ts,
+              ProofBuilder pc xs
+              -> getPropDef pc ds = Some (DefProp pc ts)
+              -> Forall2 (TYPE ds ke te) xs ts)
+  : exp -> exp -> Prop :=
  (* Step some sub-expression in an evaluation context *)
  | EsContext
    : forall C x x',
      exp_ctx C
-     -> STEP x x'
-     -> STEP (C x) (C x')
+     -> STEP ProofBuilder ds ProofBuilderOK x x'
+     -> STEP ProofBuilder ds ProofBuilderOK
+            (C x) (C x')
 
  | EsFixApp
    : forall t11 t22 x12 v2,
      wnfX v2
-     -> STEP (XApp (XFix t11 t22 x12) v2)
+     -> STEP ProofBuilder ds ProofBuilderOK
+            (XApp (XFix t11 t22 x12) v2)
             (substXX 0 (XFix t11 t22 x12) (substXX 0 v2 x12))
 
  | EsTupProj
    : forall vs n v',
      Forall wnfX vs
      -> get n vs = Some v'
-     -> STEP (XProj n (XTup vs)) v'
+     -> STEP ProofBuilder ds ProofBuilderOK
+            (XProj n (XTup vs)) v'
 
  | EsNFunApp
    : forall x vs ts,
      Forall wnfX vs
-     -> STEP (XNApp (XNFun ts x) vs)
+     -> STEP ProofBuilder ds ProofBuilderOK
+            (XNApp (XNFun ts x) vs)
             (substXXs 0 vs x)
 
  (* Match branching. *)
@@ -93,44 +105,37 @@ Inductive STEP : exp -> exp -> Prop :=
    : forall dc ts vs alts x,
      Forall wnfX vs
      -> getAlt dc alts = Some (AAlt dc ts x)
-     -> STEP (XMatch (XCon dc vs) alts)
+     -> STEP ProofBuilder ds ProofBuilderOK
+            (XMatch (XCon dc vs) alts)
             (substXXs 0 vs x)
 
  | EsChoice
-   : forall ds t pfc vs v tsArgs prc proofs,
-     Forall wnfX vs
-     (* get definition of proof constructor *)
-     -> getProofDef pfc ds = Some (DefProof pfc tsArgs (TProp prc))
-     (* get definition of proposition that choice proof must construct *)
-     -> getPropDef prc ds = Some (DefPropType prc proofs)
-     (* check that choice's proof inhabits the proposition it claims to inhabit *)
-     -> In pfc proofs
-     -> get 0 vs = Some v
-     (* Note: this stepping rule admits many steps we don't want *)
-     -> STEP (XChoice t pfc vs) v.
-
+   : forall pc v vs t,
+     Forall wnfX (v :: vs)
+    -> ProofBuilder pc (v :: vs)
+    -> STEP ProofBuilder ds ProofBuilderOK (XChoice t pc vs) v.
 Hint Constructors STEP.
 
 Lemma step_context_XCon_exists
- :  forall  C x dc
- ,  exps_ctx wnfX C
- -> (exists x', STEP x x')
- -> (exists x', STEP (XCon dc (C x)) (XCon dc (C x'))).
+  : forall pb ds pbOK C x dc,
+    exps_ctx wnfX C
+    -> (exists x', STEP pb ds pbOK x x')
+    -> (exists x', STEP pb ds pbOK (XCon dc (C x)) (XCon dc (C x'))).
 Proof.
- intros C x dc HC HS.
+ intros pb ds pbOK C x dc HC HS.
  shift x'.
- eapply (EsContext (fun xx => XCon dc (C xx))); auto.
+ eapply (EsContext pb ds pbOK (fun xx => XCon dc (C xx))); auto.
 Qed.
 
 Lemma step_context_XTup_exists
-  : forall C x,
+  : forall pb ds pbOK C x,
     exps_ctx wnfX C
-    -> (exists x', STEP x x')
-    -> (exists x', STEP (XTup (C x)) (XTup (C x'))).
+    -> (exists x', STEP pb ds pbOK x x')
+    -> (exists x', STEP pb ds pbOK (XTup (C x)) (XTup (C x'))).
 Proof.
- intros C x HC HS.
+ intros pb ds pbOK C x HC HS.
  shift x'.
- eapply (EsContext (fun xx => XTup (C xx))); auto.
+ eapply (EsContext pb ds pbOK (fun xx => XTup (C xx))); auto.
 Qed.
 
 (* Lemma step_context_XNApp_exists *)
@@ -146,132 +151,146 @@ Qed.
 (* Qed. *)
 
 (* Small step program evaluation *)
-Inductive STEPP : prog -> prog -> Prop :=
+Inductive STEPP
+          (ProofBuilder : propcon -> list exp -> Prop)
+          (ds : defs)
+          (ProofBuilderOK : forall ke te pc xs ts,
+              ProofBuilder pc xs
+              -> getPropDef pc ds = Some (DefProp pc ts)
+              -> Forall2 (TYPE ds ke te) xs ts)
+  : prog -> prog -> Prop :=
 | SP_Prog : forall r x s p,
     (* STEPP (PLET (IADT r x s) p) (substTP 0 r (substXP 0 x p)) *)
-    STEPP (PLET (IADT r x s) p) (substXP 0 x (substTP 0 r p))
-| SP_Exp  : forall x x',
-    STEP x x'
-    -> STEPP (PEXP x) (PEXP x').
-
+    STEPP
+      ProofBuilder ds ProofBuilderOK
+      (PLET (IADT r x s) p)
+      (substXP 0 x (substTP 0 r p))
+| SP_Exp : forall x x',
+    STEP
+      ProofBuilder ds ProofBuilderOK
+      x x'
+    -> STEPP
+        ProofBuilder ds ProofBuilderOK
+        (PEXP x) (PEXP x').
 Hint Constructors STEPP.
 
-(********************************************************************)
-(* Multi-step evaluation.
-   A sequence of small step transitions.
-   As opposed to STEPSL, this version has an append constructor
-   ESAppend that makes it easy to join two evaluations together.
-   We use this when converting big-step evaluations to small-step.
- *)
-Inductive STEPS : exp -> exp -> Prop :=
 
- (* After no steps, we get the same exp.
-    We need this constructor to match the EVDone constructor
-    in the big-step evaluation, so we can convert between big-step
-    and multi-step evaluations. *)
- | ESNone
-   :  forall x1
-   ,  STEPS x1 x1
+(* (********************************************************************) *)
+(* (* Multi-step evaluation. *)
+(*    A sequence of small step transitions. *)
+(*    As opposed to STEPSL, this version has an append constructor *)
+(*    ESAppend that makes it easy to join two evaluations together. *)
+(*    We use this when converting big-step evaluations to small-step. *)
+(*  *) *)
+(* Inductive STEPS : exp -> exp -> Prop := *)
 
- (* Take a single step. *)
- | ESStep
-   :  forall x1 x2
-   ,  STEP  x1 x2
-   -> STEPS x1 x2
+(*  (* After no steps, we get the same exp. *)
+(*     We need this constructor to match the EVDone constructor *)
+(*     in the big-step evaluation, so we can convert between big-step *)
+(*     and multi-step evaluations. *) *)
+(*  | ESNone *)
+(*    :  forall x1 *)
+(*    ,  STEPS x1 x1 *)
 
- (* Combine two evaluations into a third. *)
- | ESAppend
-   :  forall x1 x2 x3
-   ,  STEPS x1 x2 -> STEPS x2 x3
-   -> STEPS x1 x3.
+(*  (* Take a single step. *) *)
+(*  | ESStep *)
+(*    :  forall x1 x2 *)
+(*    ,  STEP  x1 x2 *)
+(*    -> STEPS x1 x2 *)
 
-Hint Constructors STEPS.
+(*  (* Combine two evaluations into a third. *) *)
+(*  | ESAppend *)
+(*    :  forall x1 x2 x3 *)
+(*    ,  STEPS x1 x2 -> STEPS x2 x3 *)
+(*    -> STEPS x1 x3. *)
+
+(* Hint Constructors STEPS. *)
 
 
-(* Context lemmas
-   These help when proving something about a reduction in a given
-   context. They're all trivial.
-   TODO: Define contexts directly like in the Simple proof.
- *)
-(* Lemma steps_app1 *)
-(*  :  forall x1 x1' x2 *)
-(*  ,  STEPS x1 x1' *)
-(*  -> STEPS (XApp x1 x2) (XApp x1' x2). *)
+(* (* Context lemmas *)
+(*    These help when proving something about a reduction in a given *)
+(*    context. They're all trivial. *)
+(*    TODO: Define contexts directly like in the Simple proof. *)
+(*  *) *)
+(* (* Lemma steps_app1 *) *)
+(* (*  :  forall x1 x1' x2 *) *)
+(* (*  ,  STEPS x1 x1' *) *)
+(* (*  -> STEPS (XApp x1 x2) (XApp x1' x2). *) *)
+(* (* Proof. *) *)
+(* (*  intros. induction H; eauto. *) *)
+(* (* Qed. *) *)
+(* (* Hint Resolve steps_app1. *) *)
+
+
+(* (* Lemma steps_app2 *) *)
+(* (*  :  forall v1 x2 x2' *) *)
+(* (*  ,  value v1 *) *)
+(* (*  -> STEPS x2 x2' *) *)
+(* (*  -> STEPS (XApp v1 x2) (XApp v1 x2'). *) *)
+(* (* Proof. *) *)
+(* (*  intros. induction H0; eauto. *) *)
+(* (* Qed. *) *)
+(* (* Hint Resolve steps_app2. *) *)
+
+
+(* (* Lemma steps_APP1 *) *)
+(* (*  :  forall x1 x1' t2 *) *)
+(* (*  ,  STEPS x1 x1' *) *)
+(* (*  -> STEPS (XAPP x1 t2) (XAPP x1' t2). *) *)
+(* (* Proof. *) *)
+(* (*  intros. induction H; eauto. *) *)
+(* (* Qed. *) *)
+
+
+(* (********************************************************************) *)
+(* (* Left linearised multi-step evaluation *)
+(*    As opposed to STEPS, this version provides a single step at a time *)
+(*    and does not have an append constructor. This is convenient *)
+(*    when converting a small-step evaluations to big-step, via the *)
+(*    eval_expansion lemma. *)
+(*  *) *)
+(* Inductive STEPSL : exp -> exp -> Prop := *)
+
+(*  | ESLNone *)
+(*    : forall x1 *)
+(*    , STEPSL x1 x1 *)
+
+(*  | ESLCons *)
+(*    :  forall x1 x2 x3 *)
+(*    ,  STEP   x1 x2 -> STEPSL x2 x3 *)
+(*    -> STEPSL x1 x3. *)
+
+(* Hint Constructors STEPSL. *)
+
+
+(* (* Transitivity of left linearised multi-step evaluation. *)
+(*    We use this when "flattening" a big step evaluation to the *)
+(*    small step one. *)
+(*  *) *)
+(* Lemma stepsl_trans *)
+(*  :  forall x1 x2 x3 *)
+(*  ,  STEPSL x1 x2 -> STEPSL x2 x3 *)
+(*  -> STEPSL x1 x3. *)
 (* Proof. *)
-(*  intros. induction H; eauto. *)
+(*  intros. *)
+(*  induction H. *)
+(*   eauto. *)
+(*   eapply ESLCons. eauto. eauto. *)
 (* Qed. *)
-(* Hint Resolve steps_app1. *)
 
 
-(* Lemma steps_app2 *)
-(*  :  forall v1 x2 x2' *)
-(*  ,  value v1 *)
-(*  -> STEPS x2 x2' *)
-(*  -> STEPS (XApp v1 x2) (XApp v1 x2'). *)
+(* (* Linearise a regular multi-step evaluation. *)
+(*    This flattens out all the append constructors, leaving us with *)
+(*    a list of individual transitions. *)
+(*  *) *)
+(* Lemma stepsl_of_steps *)
+(*  :  forall x1 x2 *)
+(*  ,  STEPS  x1 x2 *)
+(*  -> STEPSL x1 x2. *)
 (* Proof. *)
-(*  intros. induction H0; eauto. *)
+(*  intros. *)
+(*  induction H. *)
+(*   auto. *)
+(*   eauto. *)
+(*   eapply stepsl_trans; eauto. *)
 (* Qed. *)
-(* Hint Resolve steps_app2. *)
-
-
-(* Lemma steps_APP1 *)
-(*  :  forall x1 x1' t2 *)
-(*  ,  STEPS x1 x1' *)
-(*  -> STEPS (XAPP x1 t2) (XAPP x1' t2). *)
-(* Proof. *)
-(*  intros. induction H; eauto. *)
-(* Qed. *)
-
-
-(********************************************************************)
-(* Left linearised multi-step evaluation
-   As opposed to STEPS, this version provides a single step at a time
-   and does not have an append constructor. This is convenient
-   when converting a small-step evaluations to big-step, via the
-   eval_expansion lemma.
- *)
-Inductive STEPSL : exp -> exp -> Prop :=
-
- | ESLNone
-   : forall x1
-   , STEPSL x1 x1
-
- | ESLCons
-   :  forall x1 x2 x3
-   ,  STEP   x1 x2 -> STEPSL x2 x3
-   -> STEPSL x1 x3.
-
-Hint Constructors STEPSL.
-
-
-(* Transitivity of left linearised multi-step evaluation.
-   We use this when "flattening" a big step evaluation to the
-   small step one.
- *)
-Lemma stepsl_trans
- :  forall x1 x2 x3
- ,  STEPSL x1 x2 -> STEPSL x2 x3
- -> STEPSL x1 x3.
-Proof.
- intros.
- induction H.
-  eauto.
-  eapply ESLCons. eauto. eauto.
-Qed.
-
-
-(* Linearise a regular multi-step evaluation.
-   This flattens out all the append constructors, leaving us with
-   a list of individual transitions.
- *)
-Lemma stepsl_of_steps
- :  forall x1 x2
- ,  STEPS  x1 x2
- -> STEPSL x1 x2.
-Proof.
- intros.
- induction H.
-  auto.
-  eauto.
-  eapply stepsl_trans; eauto.
-Qed.
