FiatFormal/Language/PreservationP.v
@@ -10,13 +10,13 @@ Require Import FiatFormal.Language.Preservation.
 
 (* When a closed program takes a step the result has the same type. *)
 Theorem preservationP
- :  forall ds p p' t
- ,  TYPEPROG ds nil nil p t
- -> STEPP p p'
- -> TYPEPROG ds nil nil p' t.
+  : forall pb ds pbOK p p' t,
+    TYPEPROG ds nil nil p t
+    -> STEPP pb ds pbOK p p'
+    -> TYPEPROG ds nil nil p' t.
 Proof.
-  intros ds p p' t HT HS.
-  gen ds p' t.
+  intros pb ds pbOK p p' t HT HS.
+  gen pb ds pbOK p' t.
   induction p; intros.
   Case "PLet".
   invert HS; intros.
@@ -30,39 +30,39 @@ Proof.
   invert HS; intros; subst.
   invert HT; intros; subst.
   apply TYExp.
-  apply (preservation _ _ _ _ H4 H0).
+  apply (preservation _ _ _ _ _ _ H4 H0).
 Qed.
 
 
-(* When we multi-step evaluate some expression,
-   then the result has the same type as the original.
- *)
-Lemma preservation_steps
-  : forall ds x1 t1 x2,
-    TYPE ds nil nil x1 t1
-    -> STEPS x1 x2
-    -> TYPE ds nil nil x2 t1.
-Proof.
- intros.
- induction H0; eauto.
-  eapply preservation; eauto.
-Qed.
+(* (* When we multi-step evaluate some expression, *)
+(*    then the result has the same type as the original. *)
+(*  *) *)
+(* Lemma preservation_steps *)
+(*   : forall ds x1 t1 x2, *)
+(*     TYPE ds nil nil x1 t1 *)
+(*     -> STEPS x1 x2 *)
+(*     -> TYPE ds nil nil x2 t1. *)
+(* Proof. *)
+(*  intros. *)
+(*  induction H0; eauto. *)
+(*   eapply preservation; eauto. *)
+(* Qed. *)
 
 
-(* When we multi-step evaluate some expression,
-   then the result has the same type as the original.
-   Using the left-linearised form for the evaluation.
- *)
-Lemma preservation_stepsl
-  : forall ds x1 t1 x2,
-    TYPE ds nil nil x1 t1
-    -> STEPSL x1 x2
-    -> TYPE ds nil nil x2 t1.
-Proof.
- intros.
- induction H0.
-  auto.
-  apply IHSTEPSL.
-  eapply preservation.
-   eauto. auto.
-Qed.
+(* (* When we multi-step evaluate some expression, *)
+(*    then the result has the same type as the original. *)
+(*    Using the left-linearised form for the evaluation. *)
+(*  *) *)
+(* Lemma preservation_stepsl *)
+(*   : forall ds x1 t1 x2, *)
+(*     TYPE ds nil nil x1 t1 *)
+(*     -> STEPSL x1 x2 *)
+(*     -> TYPE ds nil nil x2 t1. *)
+(* Proof. *)
+(*  intros. *)
+(*  induction H0. *)
+(*   auto. *)
+(*   apply IHSTEPSL. *)
+(*   eapply preservation. *)
+(*    eauto. auto. *)
+(* Qed. *)
