FiatFormal/Language/Progress.v
@@ -1,4 +1,3 @@
-
 Require Import FiatFormal.Language.Step.
 Require Import FiatFormal.Language.SubstExpExp.
 Require Import FiatFormal.Language.SubstTypeExp.
@@ -60,7 +59,7 @@ Proof.
   intros.
   inverts H.
   pose proof @get_length_less_exists exp.
-  pose proof(Forall2_length _ _ _ H6).
+  pose proof(Forall2_length _ _ _ H5).
   apply get_length_less in H0. rewrite <- H1 in H0.
   spec H H0. dest x. eauto.
 Qed.
@@ -69,11 +68,11 @@ Qed.
 (* A well typed expression is either a value, can take a step,
    or contains a choice. *)
 Theorem progress
-  : forall ds x,
+  : forall pb ds pbOK x,
     (exists t, TYPE ds nil nil x t)
-    -> value x \/ (exists x', STEP x x') \/ hasChoiceX x.
+    -> value x \/ (exists x', STEP pb ds pbOK x x') \/ hasChoiceX x.
 Proof.
- intros. gen ds.
+ intros. gen pb ds pbOK.
  induction x using exp_mutind with
      (PA := fun a => a = a);
    rip; first [destruct H as [tx] | destruct H0 as [tx]];
@@ -86,28 +85,28 @@ Proof.
  edestruct IHx2; eauto.
  SSCase "value x2".
  pose proof (canonicalFormTFun).
- spec H1 H5. spec H1 H. destruct H1 as [x' LAM]; subst.
+ spec H1 H4. spec H1 H. destruct H1 as [x' LAM]; subst.
  SSSCase "fix".
  left; exists (substXX 0 (XFix t11 tx x') (substXX 0 x2 x')). apply EsFixApp. inverts H0; auto.
  destruct H0 as [STx2 | HCx2].
  SSCase "x2 steps".
  destruct STx2 as [x2'].
- left; exists (XApp x1 x2'). auto.
+ left; exists (XApp x1 x2'). eauto.
  SSCase "x2 hasChoice".
  right; auto.
  destruct H as [STx1 | HCx1].
  SCase "x1 steps".
  destruct STx1 as [x1'].
  left; exists (XApp x1' x2).
- eapply (EsContext (fun xx => XApp xx x2)); auto.
+ eapply (EsContext pb ds pbOK (fun xx => XApp xx x2)); eauto.
  SCase "x1 hasChoice".
  right; auto.
 
  Case "XTup".
- assert (Forall (fun x => wnfX x \/ (exists x', STEP x x') \/ hasChoiceX x) xs) as HWS.
+ assert (Forall (fun x => wnfX x \/ (exists x', STEP pb ds pbOK x x') \/ hasChoiceX x) xs) as HWS.
  repeat nforall. rip.
  have (exists t, TYPE ds nil nil x t). dest t.
- have (value x \/ (exists x', STEP x x') \/ hasChoiceX x).
+ have (value x \/ (exists x', STEP pb ds pbOK x x') \/ hasChoiceX x).
  inverts H2; rip.
  inverts H3; rip.
  (* All ctor args are wnf, or there is a context where one can step *)
@@ -129,18 +128,19 @@ Proof.
  eapply In_Context; eauto.
 
  Case "XProj".
- right. destruct (IHx ds); eauto.
+ right. assert (exists t, TYPE ds nil nil x t) by eauto.
+ destruct (IHx pb ds H pbOK); eauto.
  SCase "value x".
  pose proof (canonicalFormTNProd).
- spec H0 H5. spec H0 H. dest xs; subst.
+ spec H1 H4. spec H1 H0. dest xs; subst.
  left.
- pose proof (wellTypedProjHasX _ _ _ _ _ _ _ H5 H7).
+ pose proof (wellTypedProjHasX _ _ _ _ _ _ _ H4 H6).
  dest x. exists x. apply EsTupProj; auto.
- inverts H. inverts H1; auto.
- destruct H as [STx | HCx].
+ inverts H0. inverts H2; auto.
+ destruct H0 as [STx | HCx].
  SCase "x steps".
  left. dest x'. exists (XProj n x').
- eapply (EsContext (fun xx => XProj n xx)); eauto.
+ eapply (EsContext pb ds pbOK (fun xx => XProj n xx)); eauto.
  SCase "x hasChoice".
  (* nope. *)
  right; auto.
@@ -149,15 +149,16 @@ Proof.
  left; eauto.
 
  Case "XNApp".
- right. destruct (IHx ds); eauto.
+ right. assert (exists t, TYPE ds nil nil x t) by eauto.
+ destruct (IHx pb ds H0 pbOK); eauto.
  pose proof (canonicalFormTNFun).
- spec H1 H6. spec H1 H0. dest x'; subst.
- assert (Forall (fun x => wnfX x \/ (exists x', STEP x x') \/ hasChoiceX x) xs) as HWS.
+ spec H2 H5. spec H2 H1. dest x'; subst.
+ assert (Forall (fun x => wnfX x \/ (exists x', STEP pb ds pbOK x x') \/ hasChoiceX x) xs) as HWS.
 
  repeat nforall. rip.
  have (exists t, TYPE ds nil nil x t). dest t.
- have (value x \/ (exists x', STEP x x') \/ hasChoiceX x).
- inverts H3; rip. inverts H4. inverts H3; auto.
+ have (value x \/ (exists x', STEP pb ds pbOK x x') \/ hasChoiceX x).
+ inverts H4; rip. inverts H6. auto. (* inverts H3; auto. *)
  (* All args are wnf, or there is a context where one can step *)
  lets D: (@exps_ctx_run exp exp) HWS.
  inverts D.
@@ -165,21 +166,21 @@ Proof.
  left. eauto 6.
  (* There is a context where one ctor arg can step *)
  dest C. rename x' into x''. dest x'.
- rip. destruct H4 as [STx' | HCx'].
+ rip. destruct H6 as [STx' | HCx'].
  left.
  destruct STx'.
  exists (XNApp (XNFun ts x'') (C x)).
- eapply (EsContext (fun xx => XNApp (XNFun ts x'') (C xx))).
+ eapply (EsContext pb ds pbOK (fun xx => XNApp (XNFun ts x'') (C xx))).
  apply XcNApp2; eauto. auto.
  SCase "x' hasChoice".
  right; apply HcNApp2.
  apply Exists_exists. exists x'. rip.
  eapply In_Context; eauto.
- destruct H0 as [STx | HCx].
+ destruct H1 as [STx | HCx].
  left.
  dest x'.
  exists (XNApp x' xs); eauto.
- eapply (EsContext (fun xx => XNApp xx xs)); eauto.
+ eapply (EsContext pb ds pbOK (fun xx => XNApp xx xs)); eauto.
  SCase "x hasChoice".
  right; eauto.
 
@@ -188,10 +189,10 @@ Proof.
 
  Case "XCon".
  (* All ctor args are either wnf or can step *)
- assert (Forall (fun x => wnfX x \/ (exists x', STEP x x') \/ hasChoiceX x) xs) as HWS.
+ assert (Forall (fun x => wnfX x \/ (exists x', STEP pb ds pbOK x x') \/ hasChoiceX x) xs) as HWS.
  repeat nforall. rip.
  have (exists t, TYPE ds nil nil x t). dest t.
- have (value x \/ (exists x', STEP x x') \/ hasChoiceX x).
+ have (value x \/ (exists x', STEP pb ds pbOK x x') \/ hasChoiceX x).
  inverts H2; rip.
  inverts H6; rip.
  (* All ctor args are wnf, or there is a context where one can step *)
@@ -212,25 +213,25 @@ Proof.
  eapply In_Context; eauto.
 
  Case "XMatch".
- right.
- destruct (IHx ds); eauto.
+ right. assert (exists t, TYPE ds nil nil x t) by eauto.
+ destruct (IHx pb ds H0 pbOK); eauto.
  (* have HS: (value x \/ (exists x', STEP x x')). *)
  (* inverts HS. clear IHx. *)
  SCase "x value".
  destruct x; nope.
  SSCase "XCon".
  inverts_type.
- rewrite H8 in H9. inversion H9; subst.
+ rewrite H8 in H11. inversion H11; subst.
  (* rrwrite (dcs0 = dcs). *)
  assert (exists ts x, getAlt d aa = Some (AAlt d ts x)).
  apply getAlt_exists.
- repeat nforall. spec H11 H15. auto.
+ repeat nforall. spec H10 H15. auto.
  (* have HG: (exists ts x, getAlt d aa = Some (AAlt d ts x)) *)
  (*   by burn using getAlt_exists. *)
  dest ts. dest x.
  left. exists (substXXs 0 l x). eapply EsMatchAlt.
- inverts H0. inverts H2; auto. eauto.
- destruct H0 as [STx | HCx].
+ inverts H1. inverts H3; auto. eauto.
+ destruct H1 as [STx | HCx].
  SCase "x steps".
  left; destruct STx as [x'].
  exists (XMatch x' aa).
